finish day 3

day-3/src/Main.dfy
@@ -39,6 +39,7 @@ method mapArray2<S, T>(arr: array2<S>, fn: S -> T)
       }
 
 function method minus1(x: int): int { x - 1 }
+function method plus1(x: int): int { x + 1 }
 
 method twoDArrayToRows<T>(arr: array2<T>)
   returns (result: array<array<T>>)
@@ -91,7 +92,85 @@ method filterArray<T>(arr: array<T>, fn: T -> bool)
   ensures forall i | 0 <= i < result.Length :: fn(result[i]) == true
   ensures forall i | 0 <= i < result.Length :: contains?(arr, result[i])
   ensures forall i | 0 <= i < arr.Length :: 
-      fn(arr[i]) == true ==> contains?(result, arr[i])
+      fn(arr[i]) == true ==> contains?(result, arr[i]) {
+
+        if (arr.Length == 0) {
+          result := new T[0];
+          return;
+        }
+
+        var arraySize := 0;
+        var filteredSeq : seq<T> := [];
+
+        for i := 0 to arr.Length
+        invariant |filteredSeq| == arraySize
+        invariant arraySize <= arr.Length
+        invariant arraySize <= i
+        invariant forall i | 0 <= i < |filteredSeq| :: fn(filteredSeq[i]) == true
+        invariant forall i | 0 <= i < |filteredSeq| :: 
+            contains?(arr, filteredSeq[i])
+        invariant forall j | 0 <= j < i :: 
+            fn(arr[j]) == true ==> arr[j] in filteredSeq
+        {
+          if (fn(arr[i])) {
+            arraySize := arraySize + 1;
+            filteredSeq := filteredSeq + [arr[i]];
+          }
+        }
+
+        assert forall i | 0 <= i < arr.Length :: 
+            fn(arr[i]) == true ==> arr[i] in filteredSeq;
+
+        result := new T[|filteredSeq|](
+          i requires 0 <= i < |filteredSeq| => filteredSeq[i]);
+
+        assert forall i | 0 <= i < |filteredSeq| :: result[i] == filteredSeq[i];
+        assert forall t :: t in filteredSeq ==> contains?(result, t);
+      }
+
+function flattenSeq<T>(s: seq<set<T>>): set<T> {
+  if |s| == 0 then {} else s[0] + flattenSeq(s[1..])
+}
+
+function method filterSeq<T>(s: seq<T>, fn: T --> bool): seq<T>
+  requires forall x | x in s :: fn.requires(x)
+  ensures forall x | x in filterSeq(s, fn) :: x in s
+  ensures forall i | 0 <= i < |filterSeq(s, fn)| :: fn(filterSeq(s, fn)[i]) == true
+  ensures forall i | 0 <= i < |filterSeq(s, fn)| :: filterSeq(s, fn)[i] in s
+  ensures forall i | 0 <= i < |s| :: fn(s[i]) ==> s[i] in filterSeq(s, fn)
+  {
+    if |s| == 0 then [] else (
+      if fn(s[0]) then [s[0]] + filterSeq(s[1..], fn) else filterSeq(s[1..], fn)
+    )
+  }
+
+method twoDArrayToSeqOfSeqs<T>(arr: array2<T>)
+  returns (result: seq<seq<T>>)
+  ensures |result| == arr.Length1
+  ensures forall i | 0 <= i < arr.Length1 :: |result[i]| == arr.Length0
+  ensures forall i, j | 0 <= i < arr.Length1  && 0 <= j < arr.Length0
+      :: result[i][j] == arr[j, i]
+  {
+    result := [];
+    for i := 0 to arr.Length1
+    invariant |result| == i
+    invariant forall x | 0 <= x < i :: |result[x]| == arr.Length0
+    invariant forall x, j | 0 <= x < i && 0 <= j < arr.Length0
+        :: result[x][j] == arr[j, x]
+    {
+      var line := [];
+
+      for j := 0 to arr.Length0
+      invariant |line| == j
+      invariant forall x | 0 <= x < j :: line[x] == arr[x, i]
+      {
+        line := line + [arr[j, i]];
+      }
+
+      result := result + [line];
+    }
+  }
+
 
 datatype Bit = Zero | One
 
@@ -106,6 +185,55 @@ method binaryToDecimal(binary: array<Bit>) returns (result: int) {
     }
   }
 }
+
+function method bin2DecSeq'(binary: seq<Bit>, acc: nat): nat {
+  if |binary| == 0 then acc
+  else if binary[0] == One then bin2DecSeq'(binary[1..], acc * 2 + 1)
+  else bin2DecSeq'(binary[1..], acc * 2)
+}
+
+function method bin2DecSeq(binary: seq<Bit>): nat {
+  bin2DecSeq'(binary, 0)
+}
+
+// test
+lemma bin2DecSeq6() ensures bin2DecSeq([One, One, Zero]) == 6 {}
+lemma bin2DecSeq6'() ensures bin2DecSeq([Zero, One, One, Zero]) == 6 {}
+
+method getMostCommonBitAtIndex(i: nat, s: seq<seq<Bit>>)
+  returns (result: Bit)
+  requires forall row | row in s :: i < |row|
+  {
+    var onesCount := 0;
+
+    for j := 0 to |s| {
+      var row := s[j];
+      if (row[i] == One) {
+        onesCount := onesCount + 1;
+      }
+    }
+
+    var zeroesCount := |s| - onesCount;
+
+    if onesCount >= zeroesCount {
+      result := One;
+    } else {
+      result := Zero;
+    }
+  }
+
+method getLeastCommonBitAtIndex(i: nat, s: seq<seq<Bit>>)
+  returns (result: Bit)
+  requires forall row | row in s :: i < |row|
+  {
+    var mostCommon := getMostCommonBitAtIndex(i, s);
+    if mostCommon == One {
+      result := Zero;
+    } else {
+      result := One;
+    }
+  }
+
 
 method Main() {
   var input := getInput();
@@ -134,4 +262,49 @@ method Main() {
   print "\n";
   print "gamma * epsilon: ";
   print gammaInt * epsilonInt;
+
+  var rows := twoDArrayToSeqOfSeqs(asBits);
+  var oxygenGen := rows;
+
+  for i := 0 to 12
+  invariant |oxygenGen| > 0
+  invariant forall row | row in oxygenGen :: |row| == 12
+  {
+    var targetBit := getMostCommonBitAtIndex(i, oxygenGen);
+    var next := filterSeq(oxygenGen,
+      s requires |s| == 12 => s[i] == targetBit);
+    if |next| == 0 {
+      break;
+    }
+
+    oxygenGen := next;
+  }
+
+  var co2Scrub := rows;
+
+  for i := 0 to 12
+  invariant |co2Scrub| > 0
+  invariant forall row | row in co2Scrub :: |row| == 12
+  {
+    var targetBit := getLeastCommonBitAtIndex(i, co2Scrub);
+    var next := filterSeq(co2Scrub,
+      s requires |s| == 12 => s[i] == targetBit);
+    if |next| == 0 {
+      break;
+    }
+
+    co2Scrub := next;
+  }
+
+  var firstOxy := bin2DecSeq(oxygenGen[0]);
+  var firstCo2 := bin2DecSeq(co2Scrub[0]);
+
+  print "oxygen generator: ";
+  print firstOxy;
+  print "\n";
+  print "co2 scrubber: ";
+  print firstCo2;
+  print "\n";
+  print "oxygen generator * co2 scrubber: ";
+  print firstOxy * firstCo2;
 }
